\documentclass[11pt,a4paper]{article}
\usepackage[T1]{fontenc}
\usepackage[english]{babel}
\usepackage[latin1]{inputenc}
\usepackage{graphicx}
\usepackage{amsmath,amssymb}
\usepackage{siunitx}
	\sisetup{exponent-product = \cdot}
 	\sisetup{separate-uncertainty = true}
\usepackage{booktabs}
\usepackage[font=small,labelfont=bf]{caption}
\usepackage{enumitem}

\usepackage[scr]{rsfso}
\newcommand{\Laplace}{\mathcal{L}}

\begin{document}

\title{TMA4120 - Assignment 3} 
\author{William Dugan}

\maketitle

\section*{11.1.2}
\begin{itemize}[leftmargin=4.0cm,labelsep=0.5cm]
    \item[$\cos(nx)$] $p=2\pi/n$
    \item[$\sin(nx)$] $p=2\pi/n$
    \item[$\cos(2\pi x / k)$] $p=k$
    \item[$\sin(2\pi x / k)$] $p=k$
    \item[$\cos(2\pi nx / k)$] $p=k/n$
    \item[$\sin(2\pi nx / k)$] $p=k/n$
\end{itemize}

\section*{11.1.15}
\begin{align*}
    f(x) &= x^2,\ 0<x<2\pi,\ f(x+2\pi) = f(x)\\
    a_0 &= \frac{1}{2\pi} \int_0^{2\pi}x^2dx = \frac{4\pi^3}{3} \\
    a_n &= \frac{1}{\pi} \int_0^{2\pi} x^2\cos(nx) dx \\
    &= \frac{1}{\pi} \left[
        \frac{2}{n^2}x\cos(nx) - \frac{2-(nx)^2}{n^3}\sin(nx)
    \right]_0^{2\pi} \\
    &= \frac{4}{n^2} \\
    b_n &= \frac{1}{\pi} \int_0^{2\pi} x^2\sin(nx)dx \\
    &= \frac{1}{\pi} \left[
        \frac{2}{n^2}x\sin(nx) + \frac{2-(nx)^2}{n^3}\cos(nx)
    \right]_0^{2\pi} \\
    &= - \frac{4\pi}{n} \\
    \rightarrow S_f 
    &= 4 \left[
        \frac{{\pi^2}}{3} + \sum_{n=1}^\infty \left(
            \frac{\cos(nx)}{n^2} - \frac{\pi\sin(nx)}{n}
        \right)
    \right]
\end{align*}

\section*{11.1.17}
\begin{align*}
    f(x) &=
        \left\{\begin{matrix}
        \pi+x, &-\pi<x<0 \\ 
        \pi-x, &0<x<\pi 
        \end{matrix}\right.
\end{align*}
Since $f$ is an even function, $b_n = 0.$
\begin{align*}
    a_0 &= \frac{1}{\pi} \int_0^\pi (\pi-x)dx = \frac{\pi}{2} \\
    a_n &= \frac{2}{\pi} \int_0^\pi (\pi-x)\cos(nx)dx \\
    &= \frac{2}{\pi} \left[
        (\pi-x)\frac{1}{n}\sin(nx) - \frac{1}{n^2}\cos(nx)
    \right]_0^\pi \\
    &= \frac{2}{\pi n^2} (1-\cos(n\pi)) = \frac{2(1-(-1)^n)}{\pi n^2} \\
    \rightarrow S_f 
    &= \frac{\pi}{2} + \sum_{n=1}^\infty \frac{2(1-(-1)^n)}{\pi n^2} \cos(nx)
\end{align*} 

\section*{11.1.21}
\begin{align*}
    f(x) &=
        \left\{\begin{matrix}
        -(\pi+x), &-\pi<x<0 \\ 
        \pi-x, &0<x<\pi 
        \end{matrix}\right.
\end{align*}
Since $f$ is odd, $a_0,\ a_n = 0$.
\begin{align*}
    b_n &= \frac{2}{\pi} \int_0^\pi (\pi-x)\sin(nx)dx \\
    &= \frac{2}{\pi} \left[
        -\frac{\pi-x}{n}\cos(nx) - \frac{1}{n^2}\sin(nx)
    \right]_0^\pi \\
    &= \frac{2}{n} \\
    \rightarrow S_f 
    &= \sum_{n=1}^\infty \frac{2}{n}\sin(nx)
\end{align*}

\section*{11.2.1}
\begin{itemize}[leftmargin=4.0cm,labelsep=0.5cm]
    \item[$e^x$] Neither even nor odd.
    \item[$e^{-|x|}$] Even since $e^{-|-x|}$ = $e^{-|x|}$.
    \item[$x^3\cos(nx)$] Odd since $x^3$ is odd and $\cos x$ is even.
    \item[$x^2\tan(\pi x)$] Odd since $x^2$ is even and $\tan x$ is odd.
    \item[$\sinh x - \cosh x$] Expands to $e^{-z}$ which is neither odd nor even.
\end{itemize}

\section*{11.2.10}
\begin{align*}
    f(x) &=
        \left\{\begin{matrix}
        -(4+x), &-4<x<0 \\ 
        4-x, &0<x<4 
        \end{matrix}\right.
\end{align*}
Since $f$ is odd, $a_0,\ a_n = 0$. Using $a = n\pi/4$ we get
\begin{align*}
    b_n &= \frac{1}{2} \int_0^4 (4-x)\sin(ax)dx \\
    &= \frac{1}{2} \left[
        - \frac{4-x}{a}\cos(ax) - \frac{1}{a^2}\sin(ax)
    \right]_0^4 \\
    &= \frac{2}{a} = \frac{8}{n\pi} \\
    \rightarrow S_f
    &= \sum_{n=1}^\infty \frac{8}{n\pi}\sin\left(\frac{n\pi x}{4}\right)
\end{align*}

\section*{11.2.17}
\begin{align*}
    f(x) &=
        \left\{\begin{matrix}
        1+x, &-1<x<0 \\ 
        1-x, &0<x<1 
        \end{matrix}\right.
\end{align*}
Since $f$ is even, $b_n = 0$.
\begin{align*}
    a_0 &= \int_0^1 (1-x)dx = \frac{1}{2} \\
    a_n &= 2\int_0^1 (1-x)\sin(n\pi x)dx \\
    &= 2 \left[
        \frac{1-x}{n\pi}\sin(n\pi x) - \frac{1}{(n\pi)^2}\cos(n\pi x)
    \right]_0^1 \\
    &= \frac{2(1-(-1)^n)}{(n\pi)^2} \\
    \rightarrow S_f
    &= \frac{1}{2} + \sum_{n=1}^\infty \frac{2(1-(-1)^n)}{(n\pi)^2} \cos(n\pi x)
\end{align*}

\newpage
\section*{11.2.24}
\begin{align*}
    f(x) &=
        \left\{\begin{matrix}
        0, &0<x<2 \\ 
        1, &2<x<4 
        \end{matrix}\right.
\end{align*}
We assume $f$ is periodic with $L = 4$.
\subsection*{a) Even extension}
\begin{align*}
    a_0 &= \frac{1}{4} \int_0^4 f(x)dx = \frac{1}{2} \\
    a_n &= \frac{1}{2} \int_0^4 f(x)\cos\left(\frac{n\pi x}{4}\right)dx \\
    &= \frac{1}{2} \left[
        \frac{4}{n\pi}\sin\left(\frac{n\pi x}{4}\right)
    \right]_2^4 \\
    &= \frac{2}{n\pi}\sin\left(\frac{n\pi}{2}\right) \\
    \rightarrow S_{f_1}
    &= \frac{1}{2} + \frac{2}{\pi}\sum_{n=1}^\infty \frac{
        \sin\left(\frac{n\pi}{2}\right) \cos\left(\frac{n\pi x}{4}\right)
    }{n}
\end{align*}

\subsection*{b) Odd extension}
\begin{align*}
    b_n &= \frac{1}{2} \int_2^4 \sin\left(\frac{n\pi x}{4}\right)dx \\
    &= - \frac{2}{n\pi} [\cos\left(\frac{n\pi x}{4}\right)]_2^4 \\
    &= - \frac{2 ((-1)^n - \cos\left(\frac{n\pi}{2}\right))}{n\pi} \\
    \rightarrow S_{f_2}
    &= - \frac{2}{\pi}\sum_{n=1}^\infty \frac{(-1)^n - \cos\left(\frac{n\pi}{2}\right)}{n} \sin\left(\frac{n\pi x }{4}\right)
\end{align*}

\newpage
\section*{11.2.29}
\begin{align*}
    f(x) &= \sin x,\ 0<x<\pi
\end{align*}
We assume $f$ is periodic with $L = \pi$.
\subsection*{a) Even extension}
\begin{align*}
    a_0 &= \frac{1}{\pi} \int_0^\pi \sin x dx = \frac{2}{\pi} \\
    a_n &= \frac{2}{\pi} \int_0^\pi \sin x \cos(nx)dx \\
    &= \frac{2}{\pi} \cdot \frac{1}{1-1/n^2}\left[
        -\frac{1}{n} \sin x \sin(nx) + \frac{1}{n^2}\cos x \cos(nx)
    \right]_0^\pi \\
    &= \frac{2((-1)^{n+1} -1)}{\pi(n^2-1)} \\
    \rightarrow S_{f_1} 
    &= \frac{2}{\pi} \left(
        1 + \sum_{n=1}^\infty \frac{(-1)^{n+1} -1}{n^2-1} \sin(nx)
    \right)
\end{align*}

\subsection*{b) Odd extension}
\begin{align*}
    b_n &= \frac{2}{\pi} \int_0^\pi \sin x \sin(nx) dx \\
    &= \frac{2}{\pi} \cdot \frac{n^2}{n^2-1} \left[
        -\frac{1}{n}\sin x \cos(nx) - \frac{1}{n^2}\cos x \sin(nx)
    \right]_0^\pi \\
    &= 0\ (n \neq 1)
\end{align*}
To avoid dividing by zero we calculate $b_1$ separately.
\begin{align*}
    b_1 &= \frac{2}{\pi} \int_0^\pi \sin^2 x dx 
    = \frac{1}{\pi} \int_0^\pi (1-\cos(2x))dx
    = 1 \\
    \rightarrow S_{f_2} 
    &= \sin x
\end{align*}

\section*{11.3.15}
\begin{align*}
    r(t) &= t(\pi^2 - t^2),\ -\pi<x<\pi
\end{align*}
Since $r(-t)=-r(t)$ we get a Fourier sine series $(a_0, a_n = 0)$.
\begin{align*}
    b_n &= \frac{2}{\pi} \int_{-\pi}^\pi (\pi^2 t-t^3)\sin(nx)dx = \frac{12(-1)^{n+1}}{n^3}
\end{align*}
We can write $y = y_1 + y_2 + \dots$ which yields 
\begin{align*}
    y_n''+cy_n'+y &= \frac{12(-1)^{n+1}}{n^3} \sin(nt) \\
    (-n^2A_n + cnB_n + A_n)\cos(nt) + (-n^2B_n-cnA_n+B_n)\sin(nt) &= \frac{12(-1)^{n+1}}{n^3} \sin(nt) \\
\end{align*}
Rewritten:
\begin{align*}
    \implies -n^2A_n + cnB_n + A_n &= 0
    \implies B_n = \frac{A_n(n^2-1)}{cn} \\
    \implies -n^2B_n-cnA_n+B_n &= -n^2 \frac{A_n(n^2-1)}{cn} - cnA_n + \frac{A_n(n^2-1)}{cn} \\
    &= A_n \left[
        \frac{-n^2(n^2-1)-(cn)^2+(n^2-1)}{n}
    \right] \\
    &= A_n \left[
        \frac{(n^2-1)(1-n^2)-(cn)^2}{cn}
    \right] \\
    &\left(= \frac{12(-1)^{n+1}}{n^3} \right) \\
    \implies A_n &= \frac
        {12(-1)^{n+1}c}
        {n^2[(n^2-1)(1-n^2)-(cn)^2]} \\
    B_n &= \frac
        {12(-1)^{n+1}(n^2-1)}
        {n^3[(n^2-1)(1-n^2)-(cn)^2]}
\end{align*}


\end{document}
