\documentclass[11pt,a4paper]{article}
\usepackage[T1]{fontenc}
\usepackage[english]{babel}
\usepackage[latin1]{inputenc}
\usepackage{graphicx}
\usepackage{amsmath,amssymb}
\usepackage{siunitx}
	\sisetup{exponent-product = \cdot}
 	\sisetup{separate-uncertainty = true}
\usepackage{booktabs}
\usepackage[font=small,labelfont=bf]{caption}
\usepackage{enumitem}

\usepackage[scr]{rsfso}
\newcommand{\Laplace}{\mathcal{L}}

\begin{document}

\title{TMA4120 - Assignment 2} 
\author{William Dugan}

\maketitle

\section*{6.4.4}
\begin{align*}
    y'' + 16y = 4 \delta (t-3\pi),\ y(0) = 2,\ y'(0) = 0
\end{align*}
\begin{itemize}[leftmargin=4.0cm,labelsep=0.5cm]
\item[$\Laplace$ - transform:]
    $\Laplace\{y'' + 16y\} = \Laplace\{4 \delta (t-3\pi)\} \\
    \rightarrow s^2 Y - 2s + 16Y = 4e^{-3\pi s}$ 
\item[Solve for $Y$:]
    $(s^2 + 16) Y = 4e^{-3\pi s} + 2s \\
    \rightarrow Y = \frac{4e^{-3\pi s}}{s^2 +16} + \frac{2s}{s^2 + 16}$
\item[Inverse $\Laplace$ -transform:]
    $y = \Laplace^{-1}\{Y\}
    = \sin(4(t-3\pi)) u(t-3\pi) + 2\cos 4t$
\end{itemize}

\section*{6.4.10}
\begin{align*}
    y'' + 5y' + 6y = \delta (t - \pi / 2) + u(t-\pi)\cos t,\ y(0)=0=y'(0)
\end{align*}
\begin{itemize}[leftmargin=4.0cm,labelsep=0.5cm]
\item[$\Laplace$ - transform:]
    $\Laplace\{y'' + 5y' + 6y \} = \Laplace\{\delta (t - \pi / 2) + u(t-\pi)\cos t\} \\
    \rightarrow s^2 Y + 5sY + 6Y 
    = e^{-s\pi/2} + e^{-s\pi}\Laplace\{\cos (t+\pi)\} \\
    \rightarrow (s^2+5s+6)Y = e^{-s\pi/2} - \frac{e^{-s\pi}}{s^2+1}$ 
\item[Solve for $Y$:]
    $Y = \frac{e^{-s\pi/2}}{(s+2)(s+3)} - \frac{se^{-s\pi}}{(s+2)(s+3)(s^2+1)}$
\item[Write as partial fraction:]
    $Y 
    = e^{-s\pi/2} \left[\frac{A}{s+2} + \frac{B}{s+3}\right]
    - e^{-s\pi} \left[\frac{Cs+D}{s^2+1} + \frac{E}{s+2} + \frac{F}{s+3}\right] \\
    \rightarrow A = 1,\ B = -1.\ C,\ D,\ E,\ F:\\
    \begin{bmatrix}
        1 & 0 &1  &1  &0 \\ 
        5 &1  &3  &2  &0 \\ 
        6 &5  &1  &1  &1 \\ 
        0 &6  &3  &2  &0 
    \end{bmatrix} 
    \verb|~| I_4,\ 1/10
    \begin{bmatrix}
    1\\ 1\\ -4\\ 3
    \end{bmatrix}$
\item[Inverse $\Laplace$ -transform:]
    $y = \Laplace^{-1}\{Y\}
    = u(t-\pi/2)[e^{-2(t-\pi/2)}-e^{-3(t-\pi/2)}] 
    - \frac{u(t-\pi)}{10} [\cos(t-\pi) + \sin(t-\pi) - 4e^{-2(t-\pi)}+3e{-3(t-\pi)}] 
    $
\end{itemize}

\section*{6.5.12}
\begin{align*}
    y(t) + \int_0^t y(\tau)\cosh(t-\tau)d\tau &= t + e^t \\
    y + y * \cosh(t) &= t + e^t \\ \\
    \Laplace\{y\} + \Laplace\{y\} \cdot \Laplace\{\cosh(t)\} &= \Laplace\{t+e^t\} \\
    Y + Y \Laplace\{\cosh(t)\} &= \frac{1}{s^2} + \frac{1}{s-1} \\
    Y + Y \frac{s}{s^2-1} &= \frac{1}{s^2} + \frac{1}{s-1} \\
    Y = \frac{s^2-1}{s^2(s-1)} &= \frac{1}{s^2} + \frac{1}{s} \\
    y = \Laplace^{-1}\{Y\} &= t + 1
\end{align*}

\section*{6.5.19}
\begin{align*}
    F(s) &= \frac{2\pi s}{(s^2+\pi^2)^2} = 2 \cdot \frac{\pi}{s^2+\pi^2} \cdot \frac{s}{s^2+\pi^2} \\
    \rightarrow f(t) &= 2\sin(\pi t) * \cos(\pi t) \\
    &= 2 \int_0^t \sin(\pi\tau)\cos(\pi(t-\tau))d\tau \\
    &= 2 \int_0^t \sin(\pi\tau)\cos(\pi t)\cos(\pi\tau)d\tau
        + 2 \int_0^t \sin(\pi t)\sin^2(\pi\tau)d\tau \\
    &= \dots \\
    &= t\sin t
\end{align*}

\section*{6.5.22}
\begin{align*}
    F(s) &= \frac{e^{-as}}{s(s-2)} = \frac{e^{-as}}{s} \cdot \frac{1}{s-2} \\
    \rightarrow f(t) &= u(t-a) * e^{2t} \\
    &= \int_0^t u(\tau - a)e^{2(t - \tau)}d\tau \\
    &= \int_a^t e^{2(t-\tau)}d\tau \\
    &= \frac{1}{2} u(t-a) [e^{2(t-a)} - 1]
\end{align*}

\section*{6.6.7}
\begin{align*}
    f(t) &= t^2 \sinh(2t),\ f_1(t) = \sinh(2t) \\
    \Laplace\{t^2f_1\} &= \left(- \frac{d}{ds}\right)^2 \Laplace\{f_1\} \\
    &= \left(- \frac{d}{ds}\right)^2 \frac{2}{s^2-4} \\
    &= \frac{16s^2}{(s^2-4)^3} - \frac{4}{(s^2-4)^2}
\end{align*}

\section*{6.6.17}
\begin{align*}
    F(s) &= \ln\left(\frac{s}{s-1}\right) = \ln s - \ln (s-1) \\
    \frac{d}{ds} F &= \frac{1}{s} - \frac{1}{s-1} \\
    \Laplace^{-1}\left\{\frac{1}{s} - \frac{1}{s-1}\right\} &= 1 - e^t \\
    \rightarrow f(t) &= \frac{e^t - 1}{t}
\end{align*}

\section*{6.7.4}
\begin{align*}
    y_1' &= 4y_2 - 8\cos(4t) & y_1(0) = 0 \\
    y_2' &= -3y_1 - 9\sin(4t) & y_2(0) = 3
\end{align*}
\begin{itemize}[leftmargin=4.0cm,labelsep=0.5cm]
\item[$\Laplace$ - transform:]
    \begin{align*}
        sY_1 &= 4Y_2 - \frac{8s}{s^2+16} \\
        sY_2 -3 &= -3Y_1 - \frac{36}{s^2+16}
    \end{align*}
\item[Solve for $Y$:]
    \begin{align*}
        sY_1 - 4Y_2 &= a \\
        3Y_1 + sY_2 &= 3 - \frac{36}{s^2+16} = b \\
    \end{align*}
    $\begin{bmatrix}
        s &-4  &a \\ 
        3 &s  &b 
    \end{bmatrix}
    \verb|~| \begin{bmatrix}
    1 &-4/s  &a/s \\ 
    0 &1  &c 
    \end{bmatrix}$ where $c = \frac{b-3a/s}{s+12/s}$. \\
    $\verb|~| \begin{bmatrix}
    1 &0  &a/s + 4c/s \\ 
    0 &1  &c 
    \end{bmatrix}$ \\
    \begin{align*}
        Y_2 &= \left(\frac{-36}{s^2+16}+3+\frac{24}{s^2+16}\right) \cdot \frac{1}{s+12/s}
        = \frac{3s}{s^2+16} \\
        Y_1 &= \frac{a+4Y_2}{s} = \frac{4}{s^2+16}
    \end{align*}
\item[Inverse $\Laplace$ -transform:]
    $ y_1 = \Laplace^{-1}\{Y_1\} = \sin(4t) \\
    y_2 = \Laplace^{-1}\{Y_2\} = 3\cos(4t)$
\item[Control:] 
    $y_1(0) = 0,\ y_2(0) = 3$ Ok.
\end{itemize}

\end{document}
